\documentclass[12pt]{article}
\setlength{\parindent}{0pt}
\usepackage{amsfonts}
\usepackage{amsmath}

\begin{document}


7. Prove that for any natural number $n$

$$2 + 2^2 + 2^3 + ... + 2^n = 2^{n+1} - 2$$ 


Proof: By Induction.  Let $A(n)$ be the statement...

$$2 + 2^2 + 2^3 + ... + 2^n = 2^{n+1} - 2$$ 

Then $A(1)$ is the statement...

\begin{align*}
2^1 &= 2^2 - 2\\
2 &= 2
\end{align*}

We now assume $A(n)$ and show $A(n+1)$\newline

Adding $2^{n+1}$ to both sides we get...

\begin{align*}
2 + 2^2 + 2^3 + ... + 2^n + 2^{n+1} &= 2^{n+1} - 2 + 2^{n+1}\\
&= 2(2^{n+1}) - 2\\
&= 2^{n+2} - 2
\end{align*}

which is the formula for $n+1$ in place of $n$.\newline

Hence, by the principal of mathematical induction, the statement is proved.

\end{document}